SystemFD/Metatheory/Inversion.lean
@@ -105,11 +105,32 @@ cases lem3; case _ i lem3 =>
     subst e
     apply And.intro lem2 q2
 
+
+theorem ctx_get_openm_well_typed :
+  ⊢ Γ ->
+  Γ d@ x = .openm T ->
+  Γ ⊢ #x : T ∧ Γ ⊢ T : .kind
+:= by sorry
+
+theorem ctx_get_openm :
+  ⊢ Γ ->
+  Γ.is_openm x = true ->
+  ∃ T, Γ ⊢ #x : T ∧ Γ ⊢ T : .kind
+:= by sorry
+
 theorem ctx_get_opent_kind : ⊢ Γ -> Γ d@ x = .opent t -> Γ ⊢ t : .kind := by
 intro h1 h2
 have lem1 := frame_wf_by_index x h1
 rw [h2] at lem1; cases lem1
 case _ j => apply j
+
+theorem ctx_get_term_type_kind :
+  ⊢ Γ ->
+  Γ d@ x = .term T t
+  -> Γ ⊢ T : ★ := by
+intros wΓ h;
+sorry
+
 
 theorem ctx_get_datatype_kind : ⊢ Γ -> Γ d@ x = .datatype t -> Γ ⊢ t : .kind := by
 intro h1 h2
